Added Free and Alloc

theories/Commons/Memory.v
@@ -5,62 +5,107 @@ From RSL.Commons Require Export Values.
 From stdpp Require Import gmap.
 From stdpp Require Export fin_maps.
 
+Variant mem_cell : Type :=
+  | Freed
+  | Allocated (v: val).
+
 (* [memory] is a mapping from location to a value *)
-Definition memory := (gmap loc val).
+Definition memory := (gmap loc mem_cell).
 
 Instance memory_inhabited : Inhabited memory := populate ∅.
 
 Definition get_at (addr: val) (m: memory) : option val :=
   match addr with
-  | VPtr l => m !! l
+  | VPtr l =>
+      match m !! l with
+      | None => None
+      | Some Freed => None
+      | Some (Allocated v) => Some v
+      end
   | _ => None
   end.
 
-Definition set_at (addr: val) (v: val) (m: memory) : option memory :=
+Definition update_at (addr: val) (v: mem_cell) (m: memory) : option memory :=
   match addr with
   | VPtr l =>
       match m !! l with
       | None => None
-      | Some _ => Some (<[l := v]> m)
+      | Some Freed => None
+      | Some (Allocated _) => Some (<[l := v]> m)
       end
   | _ => None
   end.
+
+Definition set_at (addr: val) (v: val) (m: memory) : option memory :=
+  update_at addr (Allocated v) m.
+
+Definition alloc_at (l: loc) (v: val) (m: memory) : option memory :=
+  match m !! l with
+  | None => Some (<[l := Allocated v]> m)
+  | Some _ => None
+  end.
+
+Definition free_at (addr: val) (m: memory) : option memory :=
+  update_at addr Freed m.
 
 Lemma get_at_union_left l (m1 m2: memory) :
   m2 !! l = None ->
   get_at (VPtr l) (m1 ∪ m2) = get_at (VPtr l) m1.
 Proof.
-  intros Hmem; simpl. by apply lookup_union_l.
+  intros Hmem. simpl. unfold memory.
+  by rewrite lookup_union_l.
 Qed.
 
 Lemma get_at_union_right l (m1 m2: memory) :
   m1 !! l = None ->
   get_at (VPtr l) (m1 ∪ m2) = get_at (VPtr l) m2.
 Proof.
-  intros Hmem; simpl. by apply lookup_union_r.
+  intros Hmem. simpl. unfold memory.
+  by rewrite lookup_union_r.
 Qed.
 
 Lemma get_at_singl l v :
-  get_at (VPtr l) {[ l := v ]} = Some v.
+  get_at (VPtr l) {[ l := Allocated v ]} = Some v.
 Proof.
-  now apply lookup_singleton_eq.
+  simpl. unfold memory.
+  by rewrite lookup_singleton_eq.
 Qed.
 
-Lemma set_at_some l v old m:
+Lemma update_at_some l v old m:
   get_at (VPtr l) m = Some old ->
-  set_at (VPtr l) v m = Some (<[l := v]> m).
+  update_at (VPtr l) v m = Some (<[l := v]> m).
 Proof.
-  unfold set_at, get_at.
+  unfold update_at, get_at.
   intros Hget.
   destruct (m !! l) as [[]|]; congruence.
 Qed.
 
-Lemma set_at_none addr v m:
+Lemma update_at_none addr v m:
   get_at addr m = None ->
-  set_at addr v m = None.
+  update_at addr v m = None.
 Proof.
-  unfold set_at, get_at.
+  unfold update_at, get_at.
   intros Hget.
-  destruct addr; auto.
-  by rewrite Hget.
+  repeat case_match; auto.
+  congruence.
+Qed.
+
+Lemma alloc_at_is_some l v m m':
+  alloc_at l v m = Some m' <->
+  m' = m ∪ {[ l := Allocated v ]} ∧ m !! l = None.
+Proof.
+  unfold alloc_at, get_at, memory.
+  split.
+  - intros Hget.
+    case_match eqn:Hin; first congruence.
+    inv Hget. split; last done.
+    replace m with (m ∪ ∅) at 1.
+    + by rewrite (insert_union_r m ∅).
+    + by apply map_union_empty.
+  - intros [Hm HnIn].
+    rewrite HnIn.
+    f_equal.
+    replace m with (m ∪ ∅).
+    + by rewrite (insert_union_r m ∅).
+    + by apply map_union_empty.
 Qed.
