theories/Logic/MemInj.v
@@ -5,7 +5,7 @@ From RSL.Commons Require Export BijSet.
 
 From RSL.Commons Require Import RegisterBank.
 
-Implicit Types (I E: gset (loc * loc)) (lt ls : loc).
+Implicit Types (I E: loc_pair) (lt ls : loc).
 
 Definition sdom E : gset loc := set_map fst E.
 Definition tdom E : gset loc := set_map snd E.
@@ -32,9 +32,25 @@ Definition mem_inj I E : rProp :=
         if (decide (ls ∈ sdom E))
         then emp
         else
-          ∃ vt vs,
-            ⌜same_val I vt vs⌟ ∗ lt →ₜ vt ∗ ls →ₛ vs
+          (freeₜ lt ∗ freeₛ ls) ∨
+          (∃ vt vs, ⌜same_val I vt vs⌟ ∗ lt →ₜ vt ∗ ls →ₛ vs)
   )%I.
+
+Definition same_args I valt vals : rProp :=
+  ⌜Forall2 (same_val I) valt vals⌟ ∗ mem_inj I ∅.
+
+Definition samer I vt vs : rProp :=
+  ∃ I', ⌜I ⊆ I'⌟ ∗ ⌜same_val I' vt vs⌟ ∗ mem_inj I' ∅.
+
+Lemma samer_mono I I' vt vs:
+  I ⊆ I' ->
+  samer I' vt vs -∗
+  samer I vt vs.
+Proof using Type.
+  iIntros (Hincl) "(%I'' & %Hinl' & Hsame & Hinj)".
+  iExists I''. iFrame. iPureIntro.
+  by transitivity I'.
+Qed.
 
 Lemma inj_empty : ⊢ mem_inj ∅ ∅.
 Proof using Type.
@@ -45,7 +61,7 @@ Proof using Type.
   - by iApply big_sepS_empty.
 Qed.
 
-Lemma inj_insert_exploit I I' E lt ls vt vs :
+Lemma inj_insert_points_to_exploit I I' E lt ls vt vs :
   I' = {[ (ls, lt) ]} ∪ I ->
   ls ∉ sdom E ->
   lt ∉ tdom E ->
@@ -62,8 +78,9 @@ Proof using Type.
     iIntros (lt' Hej).
     iDestruct (big_sepS_delete _ _ _ Hej with "Hin") as "[Hcond H]".
     rewrite decide_False; last done.
-    iDestruct "Hcond" as (vt' vs') "(_ & Ht' & Hs')".
-    by iDestruct (src_points_to_unique with "Hs Hs'") as "%Hneq".
+    iDestruct "Hcond" as "[ (Ht' & Hs') | (%vt' & %vs' & _ & Ht' & Hs')]".
+    - by iDestruct (src_points_to_freed_unique with "Hs Hs'") as "%Hneq".
+    - by iDestruct (src_points_to_unique with "Hs Hs'") as "%Hneq".
   }
 
   iAssert (⌜∀ ls', (ls', lt) ∉ I⌝)%I with "[Hin Ht]" as "%Ht".
@@ -79,8 +96,9 @@ Proof using Type.
         - by apply HE.
       }
       subst lt. exfalso. apply Hlt. apply tdom_spec. by eexists.
-    - iDestruct "Hcond" as (vt' vs') "(_ & Ht' & Hs')".
-      by iDestruct (tgt_points_to_unique with "Ht Ht'") as "%Hneq".
+    - iDestruct "Hcond" as "[ (Ht' & Hs') | (%vt' & %vs' & _ & Ht' & Hs')]".
+      + by iDestruct (tgt_points_to_freed_unique with "Ht Ht'") as "%Hneq".
+      + by iDestruct (tgt_points_to_unique with "Ht Ht'") as "%Hneq".
   }
 
   iSplitR. { iPureIntro. by apply bij_set_extend. }
@@ -89,7 +107,7 @@ Proof using Type.
   { intros [] He%elem_of_singleton Hj. inv He. by apply (Ht ls). }
   iSplitR "Hin".
   - iApply big_sepS_singleton. rewrite decide_False; last done.
-    iExists vt, vs. iFrame. iPureIntro.
+    iRight. iExists vt, vs. iFrame. iPureIntro.
     apply same_val_mono with I.
     + by apply union_subseteq_r.
     + done.
@@ -97,15 +115,15 @@ Proof using Type.
     iModIntro. iIntros ([lt'' ls''] Hin).
     case_decide.
     + by iIntros "$".
-    + iIntros "(%vt' & %vs' & %Hsame & Hcond)".
-      iExists vt', vs'. iFrame.
+    + iIntros "[Hfree | (%vt' & %vs' & %Hsame & Hcond)]". { by iLeft. }
+      iRight. iExists vt', vs'. iFrame.
       iPureIntro.
       apply same_val_mono with I.
       * by apply union_subseteq_r.
       * done.
 Qed.
 
-Lemma inj_insert I I' lt ls vt vs :
+Lemma inj_insert_points_to I I' lt ls vt vs :
   I' = {[ (ls, lt) ]} ∪ I ->
   mem_inj I ∅ -∗
   lt →ₜ vt -∗
@@ -113,51 +131,128 @@ Lemma inj_insert I I' lt ls vt vs :
   ⌜same_val I vt vs⌟ -∗
   mem_inj I' ∅.
 Proof using Type.
-  intros. apply inj_insert_exploit; by set_solver.
+  intros. apply inj_insert_points_to_exploit; by set_solver.
+Qed.
+
+Lemma inj_insert_freed_exploit I I' E lt ls :
+  I' = {[ (ls, lt) ]} ∪ I ->
+  ls ∉ sdom E ->
+  lt ∉ tdom E ->
+  mem_inj I E -∗
+  freeₜ lt -∗
+  freeₛ ls -∗
+  mem_inj I' E.
+Proof using Type.
+  iIntros (-> Hls Hlt) "(%Hbij & %HE & Hin) Ht Hs".
+
+  iAssert (⌜∀ lt', (ls, lt') ∉ I⌝)%I with "[Hin Hs]" as "%Hs".
+  {
+    iIntros (lt' Hej).
+    iDestruct (big_sepS_delete _ _ _ Hej with "Hin") as "[Hcond H]".
+    rewrite decide_False; last done.
+    iDestruct "Hcond" as "[ (Ht' & Hs') | (%vt' & %vs' & _ & Ht' & Hs')]".
+    - by iDestruct (src_freed_unique with "Hs Hs'") as "%Hneq".
+    - by iDestruct (src_points_to_freed_unique with "Hs' Hs") as "%Hneq".
+  }
+
+  iAssert (⌜∀ ls', (ls', lt) ∉ I⌝)%I with "[Hin Ht]" as "%Ht".
+  {
+    iIntros (ls' Hej).
+    iDestruct (big_sepS_delete _ _ _ Hej with "Hin") as "[Hcond H]".
+    case_decide as He.
+    - apply sdom_spec in He as [lt' Hlt'].
+      assert (Heq: lt = lt').
+      { eapply bij_set_functional.
+        - by apply Hbij.
+        - by apply Hej.
+        - by apply HE.
+      }
+      subst lt. exfalso. apply Hlt. apply tdom_spec. by eexists.
+    - iDestruct "Hcond" as "[ (Ht' & Hs') | (%vt' & %vs' & _ & Ht' & Hs')]".
+      + by iDestruct (tgt_freed_unique with "Ht Ht'") as "%Hneq".
+      + by iDestruct (tgt_points_to_freed_unique with "Ht' Ht") as "%Hneq".
+  }
+
+  iSplitR. { iPureIntro. by apply bij_set_extend. }
+  iSplitR. { iPureIntro. intros ? ?. by apply elem_of_union_r, HE. }
+  iApply big_sepS_union.
+  { intros [] He%elem_of_singleton Hj. inv He. by apply (Ht ls). }
+  iSplitR "Hin".
+  - iApply big_sepS_singleton. rewrite decide_False; last done.
+    iLeft. iFrame.
+  - iApply (big_sepS_impl with "Hin").
+    iModIntro. iIntros ([lt'' ls''] Hin).
+    case_decide.
+    + by iIntros "$".
+    + iIntros "[Hfree | (%vt' & %vs' & %Hsame & Hcond)]". { by iLeft. }
+      iRight. iExists vt', vs'. iFrame.
+      iPureIntro.
+      apply same_val_mono with I.
+      * by apply union_subseteq_r.
+      * done.
+Qed.
+
+Lemma inj_insert_freed I I' lt ls :
+  I' = {[ (ls, lt) ]} ∪ I ->
+  mem_inj I ∅ -∗
+  freeₜ lt -∗
+  freeₛ ls -∗
+  mem_inj I' ∅.
+Proof using Type.
+  intros. apply inj_insert_freed_exploit; by set_solver.
 Qed.
 
 Lemma inj_exploit I E lt ls :
   related I lt ls ->
   ls ∉ sdom E ->
   mem_inj I E -∗
-  ∃ E' vt vs,
-    lt →ₜ vt ∗
-    ls →ₛ vs ∗
-    ⌜same_val I vt vs⌟ ∗
+  ∃ E',
     ⌜E' = {[ (ls, lt) ]} ∪ E⌟ ∗
-    mem_inj I E'.
+    mem_inj I E' ∗
+    (
+      (freeₜ lt ∗ freeₛ ls)
+      ∨
+      (∃ vt vs, ⌜same_val I vt vs⌟ ∗ lt →ₜ vt ∗ ls →ₛ vs)
+    ).
 Proof using Type.
   iIntros (Hrel HnE) "(%Hbij & %HE & Hin)".
   iDestruct (big_sepS_delete _ _ _ Hrel with "Hin") as "[Hpair Hin]".
   rewrite decide_False; last done.
-  iDestruct "Hpair" as (vt vs) "(%Hsame & Ht & Hs)".
-  iExists _, vt, vs. iFrame.
-  iSplitR. { done. }
-  iSplitR. { done. }
-  iSplitR. { done. }
-  iSplitR. { iPureIntro. intros p [->%elem_of_singleton | Hin]%elem_of_union; by auto. }
-  iApply (big_sepS_delete _ _ _ Hrel).
-  iSplitR.
-  - rewrite decide_True; first done.
-    apply sdom_spec. eexists.
-    by apply elem_of_union_l, elem_of_singleton.
-  - iApply (big_sepS_impl with "Hin").
-    iModIntro.
-    iIntros ([ls' lt'] Hneq).
-    assert (ls ≠ ls') by (by eapply bij_set_diff_fst_neq).
-    case_decide as He.
-    + iIntros "_". rewrite decide_True; first done.
-      apply sdom_spec in He  as [lt'' Hin].
-      apply sdom_spec. exists lt''. by apply elem_of_union_r.
-    + iIntros "(%vt' & %vs' & Hsame & Hcond)".
-      rewrite decide_False; first iFrame.
-      intros [lt'' Hin]%sdom_spec.
-      apply elem_of_union in Hin as [Heq%elem_of_singleton | Hin ].
-      * by inv Heq.
-      * apply He, sdom_spec. by exists lt''.
+  iExists _.
+  iSplitR; [ by iPureIntro | ].
+  iSplitL "Hin".
+  {
+    iSplitR. { done. }
+    iSplitR. { iPureIntro. intros p [->%elem_of_singleton | Hin]%elem_of_union; by auto. }
+    iApply (big_sepS_delete _ _ _ Hrel).
+    iSplitR.
+    - rewrite decide_True; first done.
+      apply sdom_spec. eexists.
+      by apply elem_of_union_l, elem_of_singleton.
+    - iApply (big_sepS_impl with "Hin").
+      iModIntro.
+      iIntros ([ls' lt'] Hneq).
+      assert (ls ≠ ls') by (by eapply bij_set_diff_fst_neq).
+      case_decide as He.
+      + iIntros "_". rewrite decide_True; first done.
+        apply sdom_spec in He  as [lt'' Hin].
+        apply sdom_spec. exists lt''. by apply elem_of_union_r.
+      + assert (ls' ∉ sdom ({[(ls, lt)]} ∪ E)).
+        {
+          intros [lt'' Hin]%sdom_spec.
+          apply elem_of_union in Hin as [Heq%elem_of_singleton | Hin ].
+          - by inv Heq.
+          - apply He, sdom_spec. by exists lt''.
+        }
+        rewrite decide_False; last done.
+        iIntros "$".
+  }
+  iDestruct "Hpair" as "[H | (%vt & %vs & H)]".
+  - by iLeft.
+  - iRight. by iExists vt, vs.
 Qed.
 
-Lemma inj_release I E E' lt ls vt vs:
+Lemma inj_release_points_to I E E' lt ls vt vs:
   (ls, lt) ∈ E ->
   E' = E ∖ {[ (ls, lt) ]} ->
   same_val I vt vs ->
@@ -175,7 +270,7 @@ Proof using Type.
   iApply (big_sepS_delete _ _ _ Hin).
   iSplitL "Ht Hs".
   { rewrite decide_False.
-    - iExists vt, vs. by iFrame.
+    - iRight. iExists vt, vs. by iFrame.
     - intros [lt' [Hin' HnIn]%elem_of_difference]%sdom_spec.
       apply HnIn, elem_of_singleton. f_equal.
       by eapply bij_set_functional; eauto. }
@@ -193,12 +288,61 @@ Proof using Type.
       apply elem_of_difference. split; first done.
       intros Hcontra%elem_of_singleton.
       inv Hcontra.
-    + iIntros "(%vt' & %vs' & Hsame & H)".
-      rewrite decide_False; first iFrame.
-      intros Hcontra.
-      apply He.
-      apply sdom_spec in Hcontra as [y Hinc].
-      apply elem_of_difference in Hinc as [].
-      apply sdom_spec. by exists y.
+    + assert (ls' ∉ sdom (E ∖ {[(ls, lt)]})).
+      {
+        intros Hcontra. apply He.
+        apply sdom_spec in Hcontra as [y Hinc].
+        apply elem_of_difference in Hinc as [].
+        apply sdom_spec. by exists y.
+      }
+      rewrite decide_False; last done.
+      iIntros "$".
+  - apply sdom_spec. by eexists.
+Qed.
+
+Lemma inj_release_freed I E E' lt ls:
+  (ls, lt) ∈ E ->
+  E' = E ∖ {[ (ls, lt) ]} ->
+  mem_inj I E -∗
+  freeₜ lt -∗
+  freeₛ ls -∗
+  mem_inj I E'.
+Proof using Type.
+  iIntros (HE ->) "(%Hbij & %Hinj & Hin) Ht Hs".
+  iSplitR. { done. }
+  iSplitR.
+  { iPureIntro. intros ? [Hin ?]%elem_of_difference. by apply Hinj, Hin. }
+  assert (Hin: (ls, lt) ∈ I) by (now apply Hinj).
+  iDestruct (big_sepS_delete _ _ _ Hin with "Hin") as "[H Hin]".
+  iApply (big_sepS_delete _ _ _ Hin).
+  iSplitL "Ht Hs".
+  { rewrite decide_False.
+    - iLeft. by iFrame.
+    - intros [lt' [Hin' HnIn]%elem_of_difference]%sdom_spec.
+      apply HnIn, elem_of_singleton. f_equal.
+      by eapply bij_set_functional; eauto. }
+  iApply (big_sepS_impl with "Hin").
+  rewrite decide_True.
+  - iDestruct "H" as "_".
+    iModIntro.
+    iIntros ([ls' lt'] Hin').
+    assert (ls ≠ ls') by (by eapply bij_set_diff_fst_neq).
+    case_decide as He.
+    + iIntros "_".
+      rewrite decide_True; first done.
+      apply sdom_spec in He as [lt'' He].
+      apply sdom_spec. exists lt''.
+      apply elem_of_difference. split; first done.
+      intros Hcontra%elem_of_singleton.
+      inv Hcontra.
+    + assert (ls' ∉ sdom (E ∖ {[(ls, lt)]})).
+      {
+        intros Hcontra. apply He.
+        apply sdom_spec in Hcontra as [y Hinc].
+        apply elem_of_difference in Hinc as [].
+        apply sdom_spec. by exists y.
+      }
+      rewrite decide_False; last done.
+      iIntros "$".
   - apply sdom_spec. by eexists.
 Qed.
