theories/Logic/PointsTo.v
@@ -5,11 +5,11 @@ From RSL.Commons Require Export Memory.
 From RSL.Logic Require Export BI.
 From RSL.Logic Require Import rPropDef Tactic.
 
-Program Definition tgt_points_to  loc v : rProp :=
-  {| rProp_holds mt ms := mt = {[ loc := v ]} ∧ ms = ∅ |}.
+Program Definition tgt_points_to loc v : rProp :=
+  {| rProp_holds mt ms := mt = {[ loc := Allocated v ]} ∧ ms = ∅ |}.
 
 Program Definition src_points_to loc v : rProp :=
-  {| rProp_holds mt ms := mt = ∅ ∧ ms = {[ loc := v ]} |}.
+  {| rProp_holds mt ms := mt = ∅ ∧ ms = {[ loc := Allocated v ]} |}.
 
 Notation "l '→ₜ' v" :=
   (tgt_points_to l%positive v%Z)
@@ -19,15 +19,26 @@ Notation "l '→ₛ' v" :=
   (src_points_to l%positive v%Z)
     (at level 70, no associativity, format "l →ₛ v") : bi_scope.
 
-From Ltac2 Require Import Ltac2 Printf.
+Program Definition tgt_freed loc : rProp :=
+  {| rProp_holds mt ms := mt = {[ loc := Freed ]} ∧ ms = ∅ |}.
 
-Lemma tgt_points_to_unique lt1 lt2 v1 v2:
-  lt1 →ₜ v1 -∗
-  lt2 →ₜ v2 -∗
-  ⌜lt1 ≠ lt2⌝.
+Program Definition src_freed loc : rProp :=
+  {| rProp_holds mt ms := mt = ∅ ∧ ms = {[ loc := Freed ]} |}.
+
+Notation "'freeₜ' l" :=
+  (tgt_freed l%positive)
+    (at level 70) : bi_scope.
+
+Notation "'freeₛ' l" :=
+  (src_freed l%positive)
+    (at level 70) : bi_scope.
+
+Lemma tgt_points_to_unique l1 l2 v1 v2:
+  l1 →ₜ v1 -∗
+  l2 →ₜ v2 -∗
+  ⌜l1 ≠ l2⌝.
 Proof.
-  unfold tgt_points_to, src_points_to.
-  unseal. simpl.
+  unfold tgt_points_to, src_points_to, tgt_freed, src_freed.
   unseal.
   intros ? ? [-> ->] ? ? _ _ [H1 ->] ? ? Hd _ [H2 _] ->.
   apply map_disjoint_union_r in Hd as [_ Hd].
@@ -35,13 +46,65 @@ Proof.
   eapply Hd; eapply elem_of_dom, lookup_singleton_is_Some; reflexivity.
 Qed.
 
-Lemma src_points_to_unique ls1 ls2 v1 v2:
-  ls1 →ₛ v1 -∗
-  ls2 →ₛ v2 -∗
-  ⌜ls1 ≠ ls2⌝.
+Lemma tgt_freed_unique l1 l2:
+  freeₜ l1 -∗
+  freeₜ l2 -∗
+  ⌜l1 ≠ l2⌝.
+Proof.
+  unfold tgt_points_to, src_points_to, tgt_freed, src_freed.
+  unseal.
+  intros ? ? [-> ->] ? ? _ _ [H1 ->] ? ? Hd _ [H2 _] ->.
+  apply map_disjoint_union_r in Hd as [_ Hd].
+  apply map_disjoint_dom in Hd. subst.
+  eapply Hd; eapply elem_of_dom, lookup_singleton_is_Some; reflexivity.
+Qed.
+
+Lemma tgt_points_to_freed_unique l1 l2 v:
+  l1 →ₜ v -∗
+  freeₜ l2 -∗
+  ⌜l1 ≠ l2⌝.
+Proof.
+  unfold tgt_points_to, src_points_to, tgt_freed, src_freed.
+  unseal.
+  intros ? ? [-> ->] ? ? _ _ [H1 ->] ? ? Hd _ [H2 _] ->.
+  apply map_disjoint_union_r in Hd as [_ Hd].
+  apply map_disjoint_dom in Hd. subst.
+  eapply Hd; eapply elem_of_dom, lookup_singleton_is_Some; reflexivity.
+Qed.
+
+Lemma src_points_to_unique l1 l2 v1 v2:
+  l1 →ₛ v1 -∗
+  l2 →ₛ v2 -∗
+  ⌜l1 ≠ l2⌝.
 Proof.
   unfold tgt_points_to, src_points_to.
   unseal. simpl. unseal.
+  intros ? ? [-> ->] ? ? _ _ [-> H1] ? ? _ Hd [_ H2] ->.
+  apply map_disjoint_union_r in Hd as [_ Hd].
+  apply map_disjoint_dom in Hd. subst.
+  eapply Hd; eapply elem_of_dom, lookup_singleton_is_Some; reflexivity.
+Qed.
+
+Lemma src_freed_unique l1 l2:
+  freeₛ l1 -∗
+  freeₛ l2 -∗
+  ⌜l1 ≠ l2⌝.
+Proof.
+  unfold tgt_points_to, src_points_to, tgt_freed, src_freed.
+  unseal.
+  intros ? ? [-> ->] ? ? _ _ [-> H1] ? ? _ Hd [_ H2] ->.
+  apply map_disjoint_union_r in Hd as [_ Hd].
+  apply map_disjoint_dom in Hd. subst.
+  eapply Hd; eapply elem_of_dom, lookup_singleton_is_Some; reflexivity.
+Qed.
+
+Lemma src_points_to_freed_unique l1 l2 v:
+  l1 →ₛ v -∗
+  freeₛ l2 -∗
+ ⌜l1 ≠ l2⌝.
+Proof.
+  unfold tgt_points_to, src_points_to, tgt_freed, src_freed.
+  unseal.
   intros ? ? [-> ->] ? ? _ _ [-> H1] ? ? _ Hd [_ H2] ->.
   apply map_disjoint_union_r in Hd as [_ Hd].
   apply map_disjoint_dom in Hd. subst.
