theories/RTL/RTL.v
@@ -14,51 +14,57 @@ Variant op : Type :=
   | Mul
   | Div
   | Move
-  | LoadI (v: val)
+  | ImmInt (v: Z)
+  | ImmBool (v: bool)
   | Incr
   | Decr
   | EqZ.
 
 Inductive rtl_instr : Type :=
-| Inop: node -> rtl_instr
     (** No operation -- just branch to the successor. *)
-| Iop: op -> list reg -> reg -> node -> rtl_instr
+| Inop: node -> rtl_instr
     (** [Iop op args dest succ] performs the pure (not memory related)
         operation [op] over the values of registers [args],
         stores the result in [dest], and branches to [succ]. *)
-| Iload: reg -> reg -> node -> rtl_instr
+| Iop: op -> list reg -> reg -> node -> rtl_instr
     (** [Iload addr dest succ] loads the value at [addr] into [dest],
         and branches to [succ]. *)
-| Istore: reg -> reg -> node -> rtl_instr
+| Iload: reg -> reg -> node -> rtl_instr
     (** [Istore addr src succ] stores the value of register
         [src] at memory address [src], then branches to [succ]. *)
-| Icall: ident -> list reg -> reg -> node -> rtl_instr
+| Istore: reg -> reg -> node -> rtl_instr
+    (** [Ialloc dst succ] allocate a new memory cell and store the pointer into [dst],
+        and branches to [succ]. *)
+| Ialloc: reg -> node -> rtl_instr
+    (** [Ifree addr] free the address stored in [addr],
+        then branches to [succ]. *)
+| Ifree: reg -> node -> rtl_instr
     (** [Icall sig args dest succ] invokes the function determined by
         [fn], giving it the values of registers [args] as arguments.
         It stores the return value in [dest] and branches to [succ]. *)
-| Icond: reg -> node -> node -> rtl_instr
+| Icall: ident -> list reg -> reg -> node -> rtl_instr
     (** [Icond cond args ifso ifnot] branch on the value in [cond].
         If the value in register [cond] is non zero, it transitions to [ifso].
         Otherwise it transitions to [ifnot]. *)
-| Ireturn: reg -> rtl_instr
+| Icond: reg -> node -> node -> rtl_instr
     (** [Ireturn reg] terminates the execution of the current function
         (it has no successor). It returns the value of the register [reg]. *)
-.
+| Ireturn: reg -> rtl_instr.
 
 (** [code] is a finite map from nodes to rtl_instructions *)
 Definition rtl_code := gmap node rtl_instr.
 
 (** A [function] includes its signature, an entry node, and its code. *)
 Record rtl_function := {
-    fn_name: ident;
-    fn_regs: list reg;
-    fn_entrypoint : node;
-    fn_code : rtl_code;
-    fn_regs_no_dup : is_no_dup fn_regs = true;
+    rtl_fn_name: ident;
+    rtl_fn_regs: list reg;
+    rtl_fn_entrypoint : node;
+    rtl_fn_code : rtl_code;
+    rtl_fn_regs_no_dup : is_no_dup rtl_fn_regs = true;
   }.
 
 Definition find_fun_in_list (L: list rtl_function) (s: ident) : option rtl_function :=
-  snd <$> list_find (fun f => (fn_name f =? s)%string) L.
+  snd <$> list_find (fun f => (rtl_fn_name f =? s)%string) L.
 
 Record rtl_program := {
     prog_fun_list: list rtl_function;
@@ -66,7 +72,7 @@ Record rtl_program := {
     prog_main: ident;
 
     prog_fun_list_no_dup:
-      is_no_dup (fn_name <$> prog_fun_list) = true;
+      is_no_dup (rtl_fn_name <$> prog_fun_list) = true;
 
     prog_main_exists:
       is_Some (find_fun_in_list prog_fun_list prog_main);
@@ -75,9 +81,12 @@ Record rtl_program := {
 Definition find_fun (P: rtl_program) (s: ident) : option rtl_function :=
   find_fun_in_list (prog_fun_list P) s.
 
+Lemma rtl_fun_no_dup f : NoDup (rtl_fn_regs f).
+Proof using Type. by apply is_no_dup_sound, rtl_fn_regs_no_dup. Qed.
+
 (* Assert that rtl_instruction at [pc] in function [f] is [i] *)
 Notation "f '@' pc 'is' i" :=
-  ((fn_code f)!!pc = Some i) (at level 60, no associativity).
+  ((rtl_fn_code f)!!pc = Some i) (at level 60, no associativity).
 
 Definition eval_op (op: op) (args: list val) : option val :=
   match op, args with
@@ -89,7 +98,8 @@ Definition eval_op (op: op) (args: list val) : option val :=
       then None
       else Some (VInt (v1 / v2)%Z)
   | Move, [v] => Some v
-  | LoadI v, [] => Some v
+  | ImmInt v, [] => Some (VInt v)
+  | ImmBool b, [] => Some (VBool b)
   | Incr, [VInt v] => Some (VInt (v + 1)%Z)
   | Decr, [VInt v] => Some (VInt (v - 1)%Z)
   | EqZ, [VInt v] => Some (VBool (v =? 0)%Z)
