theories/Commons/Values.v
@@ -3,7 +3,7 @@ From RSL Require Import Prelude.
 From stdpp Require Import gmap.
 
 Definition loc : Type := positive.
-Definition loc_map : Type := gset (loc * loc).
+Definition loc_pair : Type := gset (loc * loc).
 
 Variant val : Type :=
 | VInt (v: Z)
@@ -11,21 +11,24 @@ Variant val : Type :=
 | VPtr (l : loc)
 | VUndef.
 
-Definition related (I: loc_map) l1 l2 :=
+Definition related (I: loc_pair) l1 l2 :=
   (l2, l1) ∈ I.
 
 Variant same_val I : val -> val -> Prop :=
-  | IntEq i1 i2:
+  | IntEq i1 i2 :
     i1 = i2 ->
     same_val I (VInt i1) (VInt i2)
 
-  | BoolEq b1 b2:
+  | BoolEq b1 b2 :
     b1 = b2 ->
     same_val I (VBool b1) (VBool b2)
 
-  | PtrEq p1 p2:
+  | PtrEq p1 p2 :
     related I p1 p2 ->
-    same_val I (VPtr p1) (VPtr p2).
+    same_val I (VPtr p1) (VPtr p2)
+
+  | UndefEq v :
+    same_val I v VUndef.
 
 Lemma same_val_mono I I' vt vs :
   I ⊆ I' ->
